\documentclass{article}
\usepackage{amsmath}
\begin{document}
\begin{equation}
    \begin{aligned}
        P_i=(x_i,y_i),(i=1,2,\dots,n)\\
        \\
        f(x_i)=ax_i + b\\     
        L(a,b)=\sum_{i=1}^n(y_i-f(x_i))^2  \\ 
        f(x)=\begin{pmatrix}
            x_i&1
        \end{pmatrix}\begin{pmatrix}
            a\\b
        \end{pmatrix}
        \begin{cases}
            f(x_1)=a x_1 +b   \\
            f(x_2)=a x_2 +b   \\
            f(x_3)=a x_3 +b   \\
            
        \end{cases} \\
        \\
        \\
        \mathbf{Y}=\begin{pmatrix}
            y_1\\y_2\\y_3
        \end{pmatrix}
        \mathbf{\hat{Y}}=\begin{pmatrix} f(x_1)\\f(x_2)\\f(x_3) \end{pmatrix}
        \mathbf{X}=\begin{pmatrix}
            x_1&1\\
            x_2&1\\
            x_3&1
        \end{pmatrix}
        \mathbf{A}=\begin{pmatrix}
            a\\b
        \end{pmatrix}\\  
        \\
        min |\mathbf{Y}-\mathbf{\hat{Y}}|^2      \\
        \\
        \mathbf{A}=(\mathbf{X}^\mathrm{T}\mathbf{X})^{-1}\mathbf{X}^\mathrm{T}\mathbf{Y}\\
        \\
        \mathbf{X}=\begin{pmatrix}
            x_1&1\\
            x_2&1\\
            x_3&1
        \end{pmatrix}=\begin{pmatrix}
            \mathbf{X}_1&\mathbf{X}_2
        \end{pmatrix}\\
        \\
        \mathbf{\hat{Y}}=\mathbf{X}\mathbf{A}\\
        \\
        \mathbf{\hat{Y}}=\mathbf{X}\mathbf{A}=\begin{pmatrix}
            \mathbf{X}_1&\mathbf{X}_2
        \end{pmatrix}\begin{pmatrix}
            a\\b
        \end{pmatrix}\\=a\mathbf{X}_1+b\mathbf{X}_2\\
        min |\mathbf{Y}-\mathbf{\hat{Y}}|^2 \to (\mathbf{Y}-\mathbf{\hat{Y}})\perp\mathbf{X_1},\mathbf{X_2}\\
        \\
        \mathbf{X_1}=\begin{pmatrix}
            x_1\\
            x_2\\
            x_3
        \end{pmatrix}
        \mathbf{X_2}=\begin{pmatrix}
            1\\
            1\\
            1
        \end{pmatrix}\\
        \mathbf{X_1}^\mathrm{T}(\mathbf{Y}-\mathbf{\hat{Y}})=\begin{pmatrix}
            x_1&x_2&x_3
        \end{pmatrix}(\mathbf{Y}-\mathbf{\hat{Y}})=0\\
        \mathbf{X_2}^\mathrm{T}(\mathbf{Y}-\mathbf{\hat{Y}})=\begin{pmatrix}
            1&1&1
        \end{pmatrix}(\mathbf{Y}-\mathbf{\hat{Y}})=0\\
        \mathbf{X}^\mathrm{T}(\mathbf{Y}-\mathbf{\hat{Y}})=0\\
        \to \begin{pmatrix}
            x_1&x_2&x_3\\
            1&1&1
        \end{pmatrix}(\mathbf{Y}-\mathbf{\hat{Y}})=0\\
        \to \mathbf{X}^\mathrm{T}(\mathbf{Y}-\mathbf{XA})=0\\
        \to \mathbf{X}^\mathrm{T}\mathbf{Y}-\mathbf{X}^\mathrm{T}\mathbf{XA}=0\\
        \to \mathbf{X}^\mathrm{T}\mathbf{Y}=\mathbf{X}^\mathrm{T}\mathbf{XA}\\
        U_0(x)=V_{k,1}^1(x)=1\\
        U_1(x)=V_{k,1}^2(x)=\sqrt{3}(1-2x),0\leq x\leq 1\\
        U_2(x)=V_{k,1}^3(x)=\sqrt{5}(6x^2-6x+1)\\
        U_3(x)=V_{k,1}^4(x)=\sqrt{7}(-20x^3+30x^2-12x+1)\\
        \mathbf{X_2}^\mathrm{T}(\mathbf{Y}-\mathbf{\hat{Y}})=\begin{pmatrix}
            1&1&1
        \end{pmatrix}(\mathbf{Y}-\mathbf{\hat{Y}})=0\\
        \mathbf{X}^\mathrm{T}(\mathbf{Y}-\mathbf{\hat{Y}})=0\\
        \to \begin{pmatrix}
            x_1&x_2&x_3\\
            1&1&1
        \end{pmatrix}(\mathbf{Y}-\mathbf{\hat{Y}})=0\\
        \to \mathbf{X}^\mathrm{T}(\mathbf{Y}-\mathbf{XA})=0\\
        \to \mathbf{X}^\mathrm{T}\mathbf{Y}-\mathbf{X}^\mathrm{T}\mathbf{XA}=0\\
        \to \mathbf{X}^\mathrm{T}\mathbf{Y}=\mathbf{X}^\mathrm{T}\mathbf{XA}\\
        U_0(x)=V_{k,1}^1(x)=1\\
        U_1(x)=V_{k,1}^2(x)=\sqrt{3}(1-2x),0\leq x\leq 1\\
        U_2(x)=V_{k,1}^3(x)=\sqrt{5}(6x^2-6x+1)\\
        U_3(x)=V_{k,1}^4(x)=\sqrt{7}(-20x^3+30x^2-12x+1)\\
        k=1:\\
        U_{1,2}^1(x)=V_{1,2}^1(x)=\left\{\begin{matrix}
        \sqrt3(-4x+1), 0\leq x< 1/2\\ 
        \sqrt3(4x-3), 1/2\leq x\leq 1
        \end{matrix}\right.\\
        U_{1,2}^2(x)=V_{1,2}^2(x)=\left\{\begin{matrix}
        -6x+1,0\leq x< 1/2\\ 
        -6x+5, 1/2\leq x\leq 1
        \end{matrix}\right.\\
        k=2:\\
        U_{2,2}^1(x)=V_{2,2}^1(x)=\left\{\begin{matrix}
        \sqrt5(16x^2-10x+1), 0\leq x< 1/2\\ 
        \sqrt5(-16x^2+22x-7), 1/2\leq x\leq 1
        \end{matrix}\right.\\
        U_{2,2}^2(x)=V_{2,2}^2(x)=\left\{\begin{matrix}
        \sqrt3(30x^2-14x+1), 0\leq x< 1/2\\ 
        \sqrt3(30x^2-46x+17), 1/2\leq x\leq 1
        \end{matrix}\right.\\
        U_{2,2}^3(x)=V_{2,2}^3(x)=\left\{\begin{matrix}
        40x^2-16x+1, 0\leq x< 1/2\\ 
        -40x^2+64x-25, 1/2\leq x\leq 1
        \end{matrix}\right.
        k=3:\\
        U_{3,2}^1(x)=V_{3,2}^1(x)=\left\{\begin{matrix}
        \sqrt7(-64x^3+66x^2-18x+1), 0\leq x< 1/2\\ 
        \sqrt7(64x^3-126x^2+78x-15), 1/2\leq x\leq 1
        \end{matrix}\right.\\
        U_{3,2}^2(x)=V_{3,2}^2(x)=\left\{\begin{matrix}
        \sqrt5(-140x^3+114x^2-24x+1), 0\leq x< 1/2\\ 
        \sqrt5(-140x^3+306x^2-216x+49), 1/2\leq x\leq 1
        \end{matrix}\right.\\
        U_{3,2}^3(x)=V_{3,2}^3(x)=\left\{\begin{matrix}
        \sqrt3(-224x^3+156x^2-28x+1), 0\leq x< 1/2\\ 
        \sqrt3(224x^3-516x^2+388x-95), 1/2\leq x\leq 1
        \end{matrix}\right.\\
        U_{3,2}^4(x)=V_{3,2}^4(x)=\left\{\begin{matrix}
        -280x^3+180x^2-30x+1, 0\leq x< 1/2\\ 
        -280x^3+660x^2-510x+129, 1/2\leq x\leq 1
        \end{matrix}\right.\\
        V_{k,n}^{i,j}=\left\{\begin{matrix}
            \sqrt{2^{n-2}}V_{k,2}^i[2^{n-2}(x-\frac{j-1}{2^{n-2}})],\frac{j-1}{2^{n-2}}<x<\frac{j}{2^{n-2}}\\ 
            0
            \end{matrix}\right.\\
    \end{aligned}   
\end{equation}
\end{document}
